projects/lib/gmp_goal_check.v
@@ -1,0 +1,6 @@
+From  Require Import gmp_goal gmp_proof_auto gmp_proof_manual.
+
+Module VC_Correctness : VC_Correct.
+  Include gmp_proof_auto.
+  Include gmp_proof_manual.
+End VC_Correctness.
