projects/lib/gmp_proof_manual.v
@@ -1,0 +1,152 @@
+Require Import Coq.ZArith.ZArith.
+Require Import Coq.Bool.Bool.
+Require Import Coq.Strings.String.
+Require Import Coq.Lists.List.
+Require Import Coq.Classes.RelationClasses.
+Require Import Coq.Classes.Morphisms.
+Require Import Coq.micromega.Psatz.
+Require Import Coq.Sorting.Permutation.
+From AUXLib Require Import int_auto Axioms Feq Idents List_lemma VMap.
+Require Import SetsClass.SetsClass. Import SetsNotation.
+From SimpleC.SL Require Import Mem SeparationLogic.
+From GmpLib Require Import gmp_goal.
+Require Import GmpLib.GmpNumber. Import Internal.
+Require Import GmpLib.GmpAux.
+Require Import Logic.LogicGenerator.demo932.Interface.
+Local Open Scope Z_scope.
+Local Open Scope sets.
+Local Open Scope string.
+Local Open Scope list.
+Import naive_C_Rules.
+Local Open Scope sac.
+
+Lemma proof_of_gmp_abs_return_wit_1_1 : gmp_abs_return_wit_1_1.
+Proof. pre_process. Qed.
+
+
+Lemma proof_of_gmp_abs_return_wit_1_2 : gmp_abs_return_wit_1_2.
+Proof. pre_process. Qed.
+
+Lemma proof_of_gmp_max_return_wit_1_1 : gmp_max_return_wit_1_1.
+Proof. 
+  pre_process.
+  entailer!.
+  unfold Zmax.
+  rewrite Z.max_r; lia.
+Qed.
+
+Lemma proof_of_gmp_max_return_wit_1_2 : gmp_max_return_wit_1_2.
+Proof.
+  pre_process.
+  entailer!.
+  unfold Zmax.
+  rewrite Z.max_l; lia.
+Qed.
+
+Lemma proof_of_gmp_cmp_return_wit_1_2 : gmp_cmp_return_wit_1_2.
+Proof.
+  pre_process.
+  repeat rewrite <-derivable1_orp_intros1.
+  entailer!.
+Qed.
+
+Lemma proof_of_mpn_copyi_entail_wit_1 : mpn_copyi_entail_wit_1.
+Proof.
+  pre_process.
+  Exists l2 l_2.
+  entailer!.
+  pose proof (Zlength_nonneg l_2).
+  lia.
+Qed.
+
+Lemma proof_of_mpn_copyi_entail_wit_2 : mpn_copyi_entail_wit_2.
+Proof.
+  pre_process.
+  Exists l2' l_3.
+  entailer!.
+  rewrite replace_Znth_app_r.
+  + rewrite Zlength_sublist0; [ | lia ].
+    assert (i - i = 0). { lia. }
+    rewrite H15; clear H15.
+    assert (replace_Znth 0 (Znth i l_3 0) (a :: nil) = sublist i (i + 1) l_3). {
+      unfold replace_Znth, Z.to_nat, replace_nth.
+      rewrite (sublist_single i l_3 0); [ reflexivity | ].
+      rewrite <-Zlength_correct; lia.
+    }
+    rewrite H15; clear H15.
+    rewrite replace_Znth_nothing.
+    - rewrite <-sublist_split; try lia; try reflexivity.
+      rewrite <-Zlength_correct; lia.
+    - pose proof (Zlength_sublist0 i l_3 ltac:(lia)).
+      lia.
+  + pose proof (Zlength_sublist0 i l_3); lia.
+Qed.
+
+Lemma proof_of_mpn_copyi_which_implies_wit_1 : mpn_copyi_which_implies_wit_1.
+Proof.
+  pre_process.
+  unfold mpd_store_Z.
+  Intros l.
+  Exists l.
+  unfold mpd_store_list.
+  entailer!.
+  subst.
+  entailer!.
+Qed.
+
+Lemma proof_of_mpn_copyi_which_implies_wit_2 : mpn_copyi_which_implies_wit_2.
+Proof.
+  pre_process.
+  pose proof (store_uint_array_divide d cap2 l2 0).
+  pose proof (Zlength_nonneg l2).
+  specialize (H0 ltac:(lia) ltac:(lia)).
+  destruct H0 as [H0 _].
+  simpl in H0.
+  entailer!.
+  rewrite (sublist_nil l2 0 0) in H0; [ | lia].
+  sep_apply H0.
+  entailer!.
+  unfold store_uint_array, store_uint_array_rec.
+  unfold store_array.
+  rewrite (sublist_self l2 cap2); [ | lia ].
+  assert (d + 0 = d). { lia. }
+  rewrite H2; clear H2.
+  assert (cap2 - 0 = cap2). { lia. }
+  rewrite H2; clear H2.
+  reflexivity.
+Qed.
+
+Lemma proof_of_mpn_copyi_which_implies_wit_3 : mpn_copyi_which_implies_wit_3.
+Proof.
+  pre_process.
+  destruct l'. {
+    unfold store_uint_array_rec.
+    simpl.
+    entailer!.
+  }
+  pose proof (store_uint_array_rec_cons d i cap2  z l' ltac:(lia)).
+  sep_apply H2.
+  Exists z l'.
+  entailer!.
+  assert (i = 0 \/ i > 0). { lia. }
+  destruct H3.
+  + subst.
+    unfold store_uint_array, store_array.
+    simpl.
+    entailer!.
+  + pose proof (Aux.store_uarray_rec_equals_store_uarray d 0 i (sublist 0 i l) ltac:(lia)).
+    destruct H4 as [_ H4].
+    assert (d + sizeof(UINT) * 0 = d). { lia. }
+    rewrite H5 in H4; clear H5.
+    assert (i - 0 = i). { lia. }
+    rewrite H5 in H4; clear H5.
+    sep_apply H4; clear H4.
+    pose proof (Aux.store_uarray_rec_equals_store_uarray d 0 (i + 1) (sublist 0 i l ++ z :: nil) ltac:(lia)).
+    destruct H4 as [H4 _].
+    assert (i + 1 - 0 = i + 1). { lia. }
+    rewrite H5 in H4; clear H5.
+    assert (d + sizeof(UINT) * 0 = d). { lia. }
+    rewrite H5 in H4; clear H5.
+    rewrite <-H4.
+    sep_apply store_uint_array_rec_tail_merge; [ reflexivity | lia ].
+Qed.
